examples/layeredeffects/ID2.fst
@@ -42,19 +42,19 @@ let run (#a:Type) (#w : w a) (c : repr a w{sat w})
   : Tot (v:a{forall p. w p ==> p v})
   = c ()
 
-let test (t : repr int (coerce_to_pure_wp (fun p -> p 42))) =
+let test (t : repr int (as_pure_wp (fun p -> p 42))) =
   let x1 = run t in
   let x2 = run t in
   assert (x1 == x2)
 
-unfold let return_wp (#a:Type) (x:a) : w a = coerce_to_pure_wp (fun p -> p x)
+unfold let return_wp (#a:Type) (x:a) : w a = as_pure_wp (fun p -> p x)
 
 let return (a : Type) (x : a) : repr a (return_wp x) =
   fun () -> x
 
 unfold let bind_wp (#a:Type) (#b:Type) (wp_f:w a) (wp_g:a -> w b) : w b =
   elim_pure_wp_monotonicity_forall ();
-  coerce_to_pure_wp (fun p -> wp_f (fun x -> wp_g x p))
+  as_pure_wp (fun p -> wp_f (fun x -> wp_g x p))
   //let aux (p1 p2 : b->Type0) : Lemma (requires (r p1 /\ r p2))
   //                                 (ensures (r (fun x -> p1 x /\ p2 x))) =
   //  calc (==>) {
@@ -89,7 +89,7 @@ let subcomp (a:Type) (wp1 wp2: w a)
 
 unfold let if_then_else_wp (#a:Type) (wp1 wp2:w a) (p:bool) : w a =
   elim_pure_wp_monotonicity_forall ();
-  coerce_to_pure_wp (fun post -> (p ==> wp1 post) /\ ((~p) ==> wp2 post))
+  as_pure_wp (fun post -> (p ==> wp1 post) /\ ((~p) ==> wp2 post))
 
 
 let if_then_else (a : Type) (wp1 wp2 : w a) (f : repr a wp1) (g : repr a wp2) (p : bool) : Type =
@@ -114,7 +114,7 @@ layered_effect {
 
 let nomon #a (w : w a) : pure_wp a =
   elim_pure_wp_monotonicity_forall ();
-  coerce_to_pure_wp (fun p -> w p)
+  as_pure_wp (fun p -> w p)
 
 let lift_pure_nd (a:Type) (wp:w a) (f:(eqtype_as_type unit -> PURE a (nomon wp))) :
   Pure (repr a wp) (requires True)
@@ -126,22 +126,22 @@ sub_effect PURE ~> ID = lift_pure_nd
 
 
 // this requires using a good if_then_else, but why?
-let rec count (n:nat) : ID int (coerce_to_pure_wp (fun p -> forall r. p r))
+let rec count (n:nat) : ID int (as_pure_wp (fun p -> forall r. p r))
  = if n = 0 then 0 else count (n-1)
 
 (* Checking that it's kind of usable *)
 
-val test_f : unit -> ID int (coerce_to_pure_wp (fun p -> p 5 /\ p 3))
+val test_f : unit -> ID int (as_pure_wp (fun p -> p 5 /\ p 3))
 let test_f () = 5
 
 // somehow needs to prove that (forall p. nomon (fun p -> p 5) p) ??
-let test_2 () : ID int (coerce_to_pure_wp (fun p -> p 5)) = 5
+let test_2 () : ID int (as_pure_wp (fun p -> p 5)) = 5
 
 let l () : int =
   reify (test_f ()) ()
 
 effect Id (a:Type) (pre:pure_pre) (post:pure_post' a pre) =
-        ID a (coerce_to_pure_wp (fun (p:pure_post a) -> pre /\ (forall (pure_result:a). post pure_result ==> p pure_result)))
+        ID a (as_pure_wp (fun (p:pure_post a) -> pre /\ (forall (pure_result:a). post pure_result ==> p pure_result)))
 
 effect IdT (a:Type) = Id a True (fun _ -> True)
 
