tests/tactics/InspectEffComp.fst
@@ -6,13 +6,13 @@ open FStar.Monotonic.Pure
 
 let test () : Type0 =
   _ by
-    (let t = (`(int -> PURE int (coerce_to_pure_wp (fun p -> p 42)))) in
+    (let t = (`(int -> PURE int (as_pure_wp (fun p -> p 42)))) in
      match inspect t with
      | Tv_Arrow bv c ->
        let c' =
          begin match inspect_comp c with
          | C_Eff us eff res args ->
-                 let args' = [(`(coerce_to_pure_wp (fun p -> p 17)), Q_Explicit)] in
+                 let args' = [(`(as_pure_wp (fun p -> p 17)), Q_Explicit)] in
                  pack_comp (C_Eff us eff res args')
          | _ -> fail "no"
          end
@@ -22,4 +22,4 @@ let test () : Type0 =
      | _ -> fail "impossible")
 
 
-let _ = assert (test () == (int -> PURE int (coerce_to_pure_wp (fun p -> p 17))))
+let _ = assert (test () == (int -> PURE int (as_pure_wp (fun p -> p 17))))
