ulib/FStar.Monotonic.Pure.fst
@@ -41,7 +41,7 @@ let intro_pure_wp_monotonicity (#a:Type) (wp:pure_wp' a)
   = reveal_opaque (`%pure_wp_monotonic) pure_wp_monotonic
 
 unfold
-let coerce_to_pure_wp (#a:Type) (wp:pure_wp' a)
+let as_pure_wp (#a:Type) (wp:pure_wp' a)
   : Pure (pure_wp a)
       (requires forall (p q:pure_post a). (forall (x:a). p x ==> q x) ==> (wp p ==> wp q))
       (ensures fun r -> r == wp)
