tests/micro-benchmarks/Unit1.UnificationTests.fst
@@ -65,24 +65,24 @@ assume val some_f (#_:squash some_predicate) (#_:unit) (_:unit) : unit
 
 open FStar.Monotonic.Pure
 
-let test_unit_valued_implicits0 () : PURE unit (coerce_to_pure_wp (fun p -> some_predicate /\ p ())) =
+let test_unit_valued_implicits0 () : PURE unit (as_pure_wp (fun p -> some_predicate /\ p ())) =
   some_f _
 
 // make sure that we are not dropping the guard
 
 [@@ expect_failure [19]]
-let test_unit_valued_implicits1 () : PURE unit (coerce_to_pure_wp (fun p -> p ())) = some_f _
+let test_unit_valued_implicits1 () : PURE unit (as_pure_wp (fun p -> p ())) = some_f _
 
 // test two refinements
 assume val some_other_predicate : prop
 assume val some_g (_:(_:unit{some_predicate}){some_other_predicate}) : unit
 
 [@@ expect_failure [19]]
-let test_unit_valued_implicits2 () : PURE unit (coerce_to_pure_wp (fun p -> p ())) = some_g _
+let test_unit_valued_implicits2 () : PURE unit (as_pure_wp (fun p -> p ())) = some_g _
 
 [@@ expect_failure [19]]
 let test_unit_valued_implicits3 ()
-: PURE unit (coerce_to_pure_wp (fun p -> some_predicate /\ p ())) = some_g _
+: PURE unit (as_pure_wp (fun p -> some_predicate /\ p ())) = some_g _
 
 let test_unit_valued_implicits4 ()
-: PURE unit (coerce_to_pure_wp (fun p -> some_predicate /\ some_other_predicate /\ p ())) = some_g _
+: PURE unit (as_pure_wp (fun p -> some_predicate /\ some_other_predicate /\ p ())) = some_g _
